FirstOrder.v
@@ -1,0 +1,139 @@
+Require Import Compare_dec.
+
+Require Import CpdtTactics.
+
+Set Implicit Arguments.
+
+Section exist.
+  Variable A : Set.
+  Variable P : A -> Prop.
+
+  Definition exists_neg : (exists i, ~ P i) -> ~ (forall j, P j) :=
+    fun (ex : exists i, ~ P i) (f : forall j, P j) =>
+      match ex with
+        | ex_intro i not_P_i => not_P_i (f i)
+      end.
+
+  Definition exists_pos : (exists i, P i) -> ~ (forall j, ~ P j) :=
+    fun (ex : exists i, P i) (f : forall j, ~ P j) =>
+      match ex with
+        | ex_intro i P_i => (f i) P_i
+      end.
+
+  Definition neg_exists : ~ (exists i, P i) -> forall j, ~ P j :=
+    fun (f : ~ (exists i, P i)) j (P_j : P j) =>
+      f (ex_intro (fun i => P i) j P_j).
+End exist.
+
+Section induction.
+  Variable P : nat -> Prop.
+  
+  Lemma sub_ind : (forall n, (forall i, i < n -> P i) -> P n) -> forall n i, i < n -> P i.
+    Hint Resolve le_lt_eq_dec : cpdt.
+    intros H n;
+      induction n;
+        [
+          crush
+          |
+            intros i j; intros;
+              assert ({i < n} + { i = n}) as dec by crush;
+                destruct dec; crush
+        ].
+  Qed.
+
+
+  Lemma ob_ind : (forall k i, i < k -> P i) -> forall n, P n.
+    intros H n; assert (n < S n) as H1 by crush; apply (H (S n) n H1).
+  Qed.
+
+  Theorem strong_ind : (forall k, (forall i, i < k -> P i) -> P k) -> forall n, P n.
+    Hint Resolve sub_ind.
+    Hint Resolve ob_ind.
+    eauto.
+  Qed.
+End induction.
+
+Definition imp_neg (A B : Prop) (f : A -> B) : ~ B -> ~ A := fun g a => g (f a).
+
+Section double_induction.
+
+  Variable P : nat -> nat -> Prop.
+
+  Lemma sub_double_ind : (forall m n, (forall i j, i < m -> j < n -> P i j) -> P m n) -> forall m n i j, i < m -> j < n -> P i j.
+    Hint Resolve le_lt_eq_dec : cpdt.
+    intros H m n;
+      induction m;
+        [
+          crush
+          |
+            induction n;
+              [
+                crush
+                |
+                  intros i j; intros;
+                    assert ({i < m} + {i = m}) as dec1 by crush;
+                      assert ({j < n} + {j = n}) as dec2 by crush;
+                        destruct dec1; destruct dec2; crush
+              ]
+        ].
+  Qed.
+
+  Lemma ob_double_ind : (forall m n i j, i < m -> j < n -> P i j) -> forall m n, P m n.
+    intros H m n;
+      assert (m < S m) as lt1 by crush;
+        assert (n < S n) as lt2 by crush;
+          apply (H (S m) (S n) m n lt1 lt2).
+  Qed.
+
+  Theorem strong_double_ind : (forall m n, (forall i j, i < m -> j < n -> P i j) -> P m n) -> forall m n, P m n.
+    Hint Resolve sub_double_ind.
+    Hint Resolve ob_double_ind.
+    eauto.
+  Qed.
+End double_induction.
+
+Section double_prop.
+  Variable A B P : nat -> nat -> Prop.
+
+  Definition prop_exists_less_pos' m n (f1 : A m n -> B m n -> P m n -> exists i, (exists j, i < m /\ j < n /\ A i j /\ B i j /\ P i j)) (f2 : forall i j, i < m -> j < n -> A i j -> B i j -> ~ P i j) (a : A m n) (b : B m n) (p : P m n) : False :=
+    match f1 a b p with
+      | ex_intro i ex_j => match ex_j with
+                             | ex_intro j c => f2 i j (proj1 c) (proj1 (proj2 c)) (proj1 (proj2 (proj2 c))) (proj1 (proj2 (proj2 (proj2 c)))) (proj2 (proj2 (proj2 (proj2 c))))
+                           end
+    end.
+
+  Definition prop_exists_less_pos (f1 : forall m n, A m n -> B m n -> P m n -> exists i, (exists j, i < m /\ j < n /\ A i j /\ B i j /\ P i j)) m n (f2 : forall i j, i < m -> j < n -> A i j -> B i j -> P i j -> False) (a : A m n) (b : B m n) (p : P m n) : False :=
+    prop_exists_less_pos' (f1 m n) f2 a b p.
+
+  Definition prop_exists_less_ind
+    (f : forall m n, A m n -> B m n -> P m n -> 
+                         exists i, (exists j, i < m /\ j < n /\ A i j /\ B i j /\ P i j))
+    : forall m n, A m n -> B m n -> P m n -> False :=
+    strong_double_ind (fun m n => A m n -> B m n -> P m n -> False) (prop_exists_less_pos f).
+
+  Definition zero_case
+    (f : forall m n, m > 0 -> n > 0 -> A m n -> B m n -> P m n ->
+                       exists i, (exists j, i < m /\ j < n /\ A i j /\ B i j /\ P i j))
+    (p0 : P 0 0 -> False)
+    (a0 : forall m, m > 0 -> A m 0 -> False)
+    (b0 : forall n, n > 0 -> B 0 n -> False)
+    m n
+    (a : A m n)
+    (b : B m n)
+    (p : P m n)
+    : exists i, (exists j, i < m /\ j < n /\ A i j /\ B i j /\ P i j).
+    induction m; induction n; crush.
+    specialize (b0 (S n)); crush.
+    specialize (a0 (S m)); crush.
+  Qed.
+
+  Definition induction :
+    (forall m n, m > 0 -> n > 0 ->
+                  A m n -> B m n -> P m n ->
+                    exists i, (exists j, i < m /\ j < n /\ A i j /\ B i j /\ P i j)) ->
+      (~ P 0 0) ->
+      (forall m, m > 0 -> ~ A m 0) ->
+      (forall n, n > 0 -> ~ B 0 n) ->
+      forall m n, A m n -> B m n -> ~ P m n :=
+    fun f p0 a0 b0 => prop_exists_less_ind (zero_case f p0 a0 b0).
+End double_prop.
